theories/wasm_interpreter_sound.v
@@ -10,8 +10,74 @@ Unset Printing Implicit Defensive.
 
 Require Import wasm wasm_opsem wasm_interpreter.
 
-Axiom run_step_soundness : forall d i s vs es s' vs' es',
-    wasm_interpreter.run_step d i (s, vs, es) = (s', vs', RS_normal es') ->
+Section Host.
+
+(* TODO: The host should be defined as a mixin. *)
+Variable mem_grow_impl : mem -> nat -> option mem.
+Hypothesis mem_grow_impl_correct :
+  forall m n m',
+    mem_grow_impl m n = Some m' ->
+    mem_grow m n = m'.
+
+Variable host_apply_impl : store_record -> function_type -> wasm.host -> list value -> option (store_record * list value).
+Hypothesis host_apply_impl_correct :
+  forall s tf h vs m',
+    host_apply_impl s tf h vs = Some m' ->
+    exists hs, wasm.host_apply s tf h vs hs = Some m'.
+
+Let run_step := run_step mem_grow_impl host_apply_impl.
+
+Lemma run_step_soundness : forall d i s vs es s' vs' es',
+    run_step d i (s, vs, es) = (s', vs', RS_normal es') ->
     exists j,
       reduce s vs es j s' vs' es'.
-(* TODO *)
+Proof.
+Admitted. (* TODO *)
+
+End Host.
+
+(* TODO: Here are all what we need to implement.
+Print Assumptions run_step.
+[[
+wasm.wasm_wrap : wasm.i64 -> wasm.i32
+wasm.wasm_promote : wasm.f32 -> wasm.f64
+wasm.wasm_extend_u : wasm.i32 -> wasm.i64
+wasm.wasm_extend_s : wasm.i32 -> wasm.i64
+wasm.wasm_deserialise : bytes -> value_type -> value
+wasm.wasm_demote : wasm.f64 -> wasm.f32
+wasm.wasm_bool : bool -> wasm.i32
+wasm.ui64_trunc_f64 : wasm.f64 -> option wasm.i64
+wasm.ui64_trunc_f32 : wasm.f32 -> option wasm.i64
+wasm.ui32_trunc_f64 : wasm.f64 -> option wasm.i32
+wasm.ui32_trunc_f32 : wasm.f32 -> option wasm.i32
+wasm.si64_trunc_f64 : wasm.f64 -> option wasm.i64
+wasm.si64_trunc_f32 : wasm.f32 -> option wasm.i64
+wasm.si32_trunc_f64 : wasm.f64 -> option wasm.i32
+wasm.si32_trunc_f32 : wasm.f32 -> option wasm.i32
+wasm.serialise_i64 : wasm.i64 -> bytes
+wasm.serialise_i32 : wasm.i32 -> bytes
+wasm.serialise_f64 : wasm.f64 -> bytes
+wasm.serialise_f32 : wasm.f32 -> bytes
+wasm.i64_r : Wasm_int.class_of wasm.i64
+wasm.i64 : eqType
+wasm.i32_r : Wasm_int.class_of wasm.i32
+wasm.i32 : eqType
+wasm.host : eqType
+wasm.f64_r : Wasm_float.class_of wasm.f64
+wasm.f64_convert_ui64 : wasm.i64 -> wasm.f64
+wasm.f64_convert_ui32 : wasm.i32 -> wasm.f64
+wasm.f64_convert_si64 : wasm.i64 -> wasm.f64
+wasm.f64_convert_si32 : wasm.i32 -> wasm.f64
+wasm.f64 : eqType
+wasm.f32_r : Wasm_float.class_of wasm.f32
+wasm.f32_convert_ui64 : wasm.i64 -> wasm.f32
+wasm.f32_convert_ui32 : wasm.i32 -> wasm.f32
+wasm.f32_convert_si64 : wasm.i64 -> wasm.f32
+wasm.f32_convert_si32 : wasm.i32 -> wasm.f32
+wasm.f32 : eqType
+eqfunction_closureP : Equality.axiom function_closure_eqb
+eqbasic_instructionP : Equality.axiom wasm.basic_instruction_eqb
+eqadministrative_instructionP : Equality.axiom administrative_instruction_eqb
+wasm.basic_instruction_eqb : basic_instruction -> basic_instruction -> bool
+]]
+*)
